[NKIFE-393] implement nested ap with reducing dimensions

KLR/Core/Indexing.lean
@@ -379,47 +379,48 @@ theorem get!_eq_comp : ∀ i : Int, start s1 s2 + step s1 s2 * i = s1.get! (s2.g
 
 end comp
 
--- /-- Defines a clipped composition operator for IndexSpans -/
--- def clipComp (s1 s2 : IndexSpan) : IndexSpan where
---   start := Int.toNat <| comp.start s1 s2
---   step := comp.step s1 s2
---   num := comp.num s1 s2
---   step_nz := Int.mul_ne_zero_iff.mpr ⟨s1.step_nz, s2.step_nz⟩
---   get_nonneg i Hlb Hub := by
---     rcases Decidable.em (0 ≤ (comp.start s1 s2)) with (H|H)
---     · rw [Int.ofNat_toNat, Int.max_eq_left H]
---       rw [comp.get!_eq_comp]
---       apply s1.get_nonneg _ _
---       · suffices comp.inbounds? s1 (s2.get! i) by
---           simp [comp.inbounds?] at this
---           apply this.2
---         unfold comp.num at Hub
---         have Hnum := @List.lenMaxPrefix_prefix_holds _ (List.range s2.num)
---                        (comp.inbounds? s1 ∘ s2.get! ∘ Int.ofNat)
---                        i.toNat ?G1 ((Int.toNat_lt Hlb).mpr Hub)
---         case G1 =>
---           apply Nat.lt_of_lt_of_le ((Int.toNat_lt Hlb).mpr Hub)
---           exact List.lenMaxPrefix_le_length
---         simp at Hnum
---         apply (Int.max_eq_left Hlb ▸ Hnum)
---       · apply s2.get_nonneg _ Hlb
---         apply Int.lt_of_lt_of_le Hub
---         apply Int.ofNat_le.mpr
---         exact comp.num_le_ub s1 s2
---     · simp only [comp.start, Int.not_le] at H
---       have _ := comp.start_neg_implies_num_zero (H := H)
---       omega
---
--- @[simp] def clipComp.wf (s1 s2 : IndexSpan) : Prop := 0 ≤ comp.start s1 s2
---
--- /-- As long as the composition is well-defined -/
--- theorem clipComp.get!_eq (s1 s2 : IndexSpan) {i} (Hwf : clipComp.wf s1 s2) :
---     (clipComp s1 s2).get! i = s1.get! (s2.get! i) := by
---   rw [← comp.get!_eq_comp]
---   simp [clipComp]
---   exact Int.max_eq_left Hwf
+/-- Defines a clipped composition operator for IndexSpans -/
+def clipComp (s1 s2 : IndexSpan) : IndexSpan where
+  start := Int.toNat <| comp.start s1 s2
+  step := comp.step s1 s2
+  num := comp.num s1 s2
+  step_nz := Int.mul_ne_zero_iff.mpr ⟨s1.step_nz, s2.step_nz⟩
+  get_nonneg i Hlb Hub := by
+    rcases Decidable.em (0 ≤ (comp.start s1 s2)) with (H|H)
+    · rw [Int.ofNat_toNat, Int.max_eq_left H]
+      rw [comp.get!_eq_comp]
+      apply s1.get_nonneg _ _
+      · suffices comp.inbounds? s1 (s2.get! i) by
+          simp [comp.inbounds?] at this
+          apply this.2
+        unfold comp.num at Hub
+        have Hnum := @List.lenMaxPrefix_prefix_holds _ (List.range s2.num)
+                       (comp.inbounds? s1 ∘ s2.get! ∘ Int.ofNat)
+                       i.toNat ?G1 ((Int.toNat_lt Hlb).mpr Hub)
+        case G1 =>
+          apply Nat.lt_of_lt_of_le ((Int.toNat_lt Hlb).mpr Hub)
+          exact List.lenMaxPrefix_le_length
+        simp at Hnum
+        apply (Int.max_eq_left Hlb ▸ Hnum)
+      · apply s2.get_nonneg _ Hlb
+        apply Int.lt_of_lt_of_le Hub
+        apply Int.ofNat_le.mpr
+        exact comp.num_le_ub s1 s2
+    · simp only [comp.start, Int.not_le] at H
+      have _ := comp.start_neg_implies_num_zero (H := H)
+      omega
+
+@[simp] def clipComp.wf (s1 s2 : IndexSpan) : Prop := 0 ≤ comp.start s1 s2
+
+/-- As long as the composition is well-defined -/
+theorem clipComp.get!_eq (s1 s2 : IndexSpan) {i} (Hwf : clipComp.wf s1 s2) :
+    (clipComp s1 s2).get! i = s1.get! (s2.get! i) := by
+  rw [← comp.get!_eq_comp]
+  simp [clipComp]
+  exact Int.max_eq_left Hwf
 
 end IndexSpan
+
 
 /- ## Layouts -/
 
@@ -428,94 +429,96 @@ structure Layout (dim : Nat) where
   offset  : Nat
   steps : List Int
   nums    : List Nat
+  offsets : List Nat
   steps_dim : steps.length = dim
   nums_dim : nums.length = dim
   deriving Repr
+--
+-- /-- An element of ℕ^dim -/
+-- structure Coord (d : Nat) where
+--   coords : List Int
+--   coords_dim : coords.length = d
+--
+-- /-- Every element of a Coord is inside the bounds of a particular shape -/
+-- def Coord.inbounds? (s : Shape) (c : Coord s.freeDim) : Prop :=
+--   (List.zip c.coords s.freeDims).Forall (fun (i, n) => 0 ≤ i ∧ i < n)
+--
+-- /-- Look up a memory coordinate in a layout, without doing any bounds checks -/
+-- def Layout.get! {d} (l : Layout d) (c : Coord d) : Int := l.offset + l.steps.dot c.coords
+--
+-- /-- A list of IndexSpans with a given dimension -/
+-- structure FreeSpans (d : Nat) where
+--   spans : List IndexSpan
+--   spans_dim : spans.length = d
+--
+-- def FreeSpans.get! {d : Nat} (f : FreeSpans d) (c : Coord d) : Coord d where
+--   coords := List.zipWith (IndexSpan.get! · ·) f.spans c.coords
+--   coords_dim := by simp [FreeSpans.spans_dim, Coord.coords_dim, Nat.min_self]
+--
+-- /- ## Composition -/
+--
+-- namespace lcomp
+--
+-- def offset {d} (f : FreeSpans d) (l : Layout d) : Int :=
+--   l.offset + l.steps.dot (f.spans.map (Int.ofNat ∘ IndexSpan.start))
+--
+-- def steps {d} (f : FreeSpans d) (l : Layout d) : List Int :=
+--   List.zipWith (· * ·) (f.spans.map IndexSpan.step) l.steps
+--
+-- structure wf {d} (f : FreeSpans d) (l : Layout d) : Prop where
+--   offset_nonneg : 0 ≤ offset f l
+--
+-- def comp {d} (f : FreeSpans d) (l : Layout d) : Layout d where
+--   offset := Int.toNat <| offset f l
+--   steps := steps f l
+--   nums  := l.nums
+--   offsets := l.offsets
+--   steps_dim := by simp [FreeSpans.spans_dim, Layout.steps_dim, Nat.min_self, steps]
+--   nums_dim := l.nums_dim
+--
+-- end lcomp
 
-/-- An element of ℕ^dim -/
-structure Coord (d : Nat) where
-  coords : List Int
-  coords_dim : coords.length = d
-
-/-- Every element of a Coord is inside the bounds of a particular shape -/
-def Coord.inbounds? (s : Shape) (c : Coord s.freeDim) : Prop :=
-  (List.zip c.coords s.freeDims).Forall (fun (i, n) => 0 ≤ i ∧ i < n)
-
-/-- Look up a memory coordinate in a layout, without doing any bounds checks -/
-def Layout.get! {d} (l : Layout d) (c : Coord d) : Int := l.offset + l.steps.dot c.coords
-
-/-- A list of IndexSpans with a given dimension -/
-structure FreeSpans (d : Nat) where
-  spans : List IndexSpan
-  spans_dim : spans.length = d
-
-def FreeSpans.get! {d : Nat} (f : FreeSpans d) (c : Coord d) : Coord d where
-  coords := List.zipWith (IndexSpan.get! · ·) f.spans c.coords
-  coords_dim := by simp [FreeSpans.spans_dim, Coord.coords_dim, Nat.min_self]
-
-/- ## Composition -/
-
-namespace lcomp
-
-def offset {d} (f : FreeSpans d) (l : Layout d) : Int :=
-  l.offset + l.steps.dot (f.spans.map (Int.ofNat ∘ IndexSpan.start))
-
-def steps {d} (f : FreeSpans d) (l : Layout d) : List Int :=
-  List.zipWith (· * ·) (f.spans.map IndexSpan.step) l.steps
-
-structure wf {d} (f : FreeSpans d) (l : Layout d) : Prop where
-  offset_nonneg : 0 ≤ offset f l
-
-def comp {d} (f : FreeSpans d) (l : Layout d) : Layout d where
-  offset := Int.toNat <| offset f l
-  steps := steps f l
-  nums  := l.nums
-  steps_dim := by simp [FreeSpans.spans_dim, Layout.steps_dim, Nat.min_self, steps]
-  nums_dim := l.nums_dim
-
-end lcomp
-
-/-- Correctness for span/layout composition
-Note that this one says nothing about staying inbounds -/
-theorem comp_get {d} (f : FreeSpans d) (l : Layout d) {c : Coord d} (Hwf : lcomp.wf f l):
-    (lcomp.comp f l).get! c = l.get! (f.get! c) := by
-  simp [lcomp.comp, Layout.get!, Int.max_eq_left Hwf.offset_nonneg]
-  unfold lcomp.offset
-  rw [Int.add_assoc]; congr 1
-  simp [FreeSpans.get!]
-  simp [lcomp.steps]
-  rcases f with ⟨L1, HL1⟩
-  rcases c with ⟨L2, HL2⟩
-  rcases l with ⟨L4, L3, L5, HL3, HL4⟩
-  simp_all
-  clear Hwf HL4 L4
-  revert L1 L3 d
-  induction L2
-  · simp
-    intro d L1 HL1 Hd L3 HL3; subst Hd
-    simp_all [List.dot]
-  · simp
-    rename_i l2 L2 IH
-    intro d L1 HL1 Hd L3 HL3; subst Hd
-    rcases L1 with _ | ⟨l1, L1⟩ ; simp at HL1
-    rcases L3 with _ | ⟨l3, L3⟩ ; simp at HL3
-    simp_all [List.dot]
-    -- Move non-recursive terms to the left
-    conv=>
-      lhs
-      rw [← Int.add_assoc]
-      enter [1]
-      rw [Int.add_assoc]
-      rw [Int.add_comm _ (_ * _ * _)]
-      rw [← Int.add_assoc]
-    conv=>
-      lhs
-      rw [Int.add_assoc]
-    -- Solve recursive and non-recursive case separately
-    congr 1
-    · rw [Int.mul_add]; congr 1
-      rw [← Int.mul_assoc, Int.mul_comm l3 _]
-    · exact IH L1 HL1 rfl _ HL3
+-- /-- Correctness for span/layout composition
+-- Note that this one says nothing about staying inbounds -/
+-- theorem comp_get {d} (f : FreeSpans d) (l : Layout d) {c : Coord d} (Hwf : lcomp.wf f l):
+--     (lcomp.comp f l).get! c = l.get! (f.get! c) := by
+--   simp [lcomp.comp, Layout.get!, Int.max_eq_left Hwf.offset_nonneg]
+--   unfold lcomp.offset
+--   rw [Int.add_assoc]; congr 1
+--   simp [FreeSpans.get!]
+--   simp [lcomp.steps]
+--   rcases f with ⟨L1, HL1⟩
+--   rcases c with ⟨L2, HL2⟩
+--   rcases l with ⟨L4, L3, L5, HL3, HL4⟩
+--   simp_all
+--   clear Hwf HL4 L4
+--   revert L1 L3 d
+--   induction L2
+--   · simp
+--     intro d L1 HL1 Hd L3 HL3; subst Hd
+--     simp_all [List.dot]
+--   · simp
+--     rename_i l2 L2 IH
+--     intro d L1 HL1 Hd L3 HL3; subst Hd
+--     rcases L1 with _ | ⟨l1, L1⟩ ; simp at HL1
+--     rcases L3 with _ | ⟨l3, L3⟩ ; simp at HL3
+--     simp_all [List.dot]
+--     -- Move non-recursive terms to the left
+--     conv=>
+--       lhs
+--       rw [← Int.add_assoc]
+--       enter [1]
+--       rw [Int.add_assoc]
+--       rw [Int.add_comm _ (_ * _ * _)]
+--       rw [← Int.add_assoc]
+--     conv=>
+--       lhs
+--       rw [Int.add_assoc]
+--     -- Solve recursive and non-recursive case separately
+--     congr 1
+--     · rw [Int.mul_add]; congr 1
+--       rw [← Int.mul_assoc, Int.mul_comm l3 _]
+--     · exact IH L1 HL1 rfl _ HL3
 
 
 /-- NOTE:
@@ -525,138 +528,140 @@ For this reason, we impose an error semantics instead. -/
 
 /- ## Span Semantics -/
 
-abbrev LayoutMap d := Layout d → Layout d
-
-def coordToIndexSpan (x : Nat) : IndexSpan where
-  start := x
-  step := 1
-  num := 1
-  step_nz := Int.zero_ne_one.symm
-  get_nonneg := by simp; omega
-
-def Slice.toIndexSpan (s : Slice) (size : Nat) : IndexSpan where
-  start := s.l
-  step := s.step
-  num := min size s.size
-  step_nz := s.wf
-  get_nonneg i := by
-    suffices 0 ≤ i → i < ↑s.size → 0 ≤ ↑s.l + s.step * i by
-      intro H1 H2; apply this H1
-      apply Int.lt_of_lt_of_le H2
-      apply Int.ofNat_le.mpr
-      exact Nat.min_le_right size s.size
-    simp [Slice.size]
-    split <;> intros Hlb Hub
-    · apply Int.le_add_of_neg_add_le_right
-      rw [Int.neg_mul_eq_neg_mul, Int.add_zero]
-      rw [← Int.toNat_of_nonneg Hlb] at Hub
-      rw [Int.mul_comm]
-      apply Int.mul_le_of_le_ediv; omega
-      rw [← Int.max_eq_left Hlb, ← Int.ofNat_toNat]
-      apply Int.le_trans (Int.le_of_lt Hub)
-      rw [Int.natCast_ediv]
-      apply Int.le_ediv_of_mul_le; omega
-      have R1 : ↑s.step.natAbs = -s.step := by
-        apply Int.ofNat_natAbs_of_nonpos; omega
-      rw [R1]; clear R1
-      apply Int.le_trans
-      · apply Int.mul_le_mul_of_nonneg_right
-        · apply Int.ediv_le_ediv
-          · omega
-          · apply Int.ofNat_le.mpr
-            exact Nat.sub_le s.l s.u
-        · omega
-      apply Int.mul_le_of_le_ediv; omega
-      apply Int.le_refl
-    · rename_i h
-      apply Int.add_nonneg (Int.ofNat_zero_le s.l)
-      apply Int.mul_nonneg (Int.not_lt.mp h) Hlb
-
-def Index.toIndexSpan (i : Index) (size : Nat) : IndexSpan :=
-  match i with
-  | .coord x => coordToIndexSpan x
-  | .slice s => s.toIndexSpan size
-
-def simpleInterpPar (t : TensorName) : IndexSpan :=
-  .full t.shape.parDim
-
-def simpleInterpFree (t : TensorName) : LayoutMap t.freeDim :=
-  let F : FreeSpans t.freeDim := ⟨t.shape.freeDims.map .full, by simp⟩
-  lcomp.comp F
-
-def basicInterpPar (b : AccessBasic) : IndexSpan :=
-  b.parIndex.toIndexSpan b.getShape.parDim
-
-def basicInterpFree (b : AccessBasic) : LayoutMap b.freeDim :=
-  let F : FreeSpans b.freeDim := FreeSpans.mk
-    (List.zipWith (·.toIndexSpan ·) b.freeIndices b.getShape.freeDims)
-    (by
-      rcases b with ⟨_, L, Hwf⟩
-      simp [AccessBasic.getShape, AccessBasic.shape]
-      apply Nat.min_eq_right
-      cases L
-      · simp at Hwf
-      · simp)
-  lcomp.comp F
-
-def patternInterpPar (p : AccessPattern) : IndexSpan :=
-  .full p.parNum
-
-def patternInterpFree (p : AccessPattern) : LayoutMap p.freeDim := fun l =>
-  let coeff_sum : Int := (p.freePattern.map APPair.step).sum
-  Layout.mk
-    (p.freeOffset + coeff_sum * l.offset).toNat
-    (l.steps.map (coeff_sum * ·))
-    (p.freePattern.map APPair.num)
-    (by rw [List.length_map]; exact l.steps_dim)
-    (by simp [List.length_map, AccessPattern.freeDim, AccessPattern.shape])
-
-def Access.interpPar : Access → IndexSpan
-| .simple s => simpleInterpPar s
-| .basic b => basicInterpPar b
-| .pattern p => patternInterpPar p
-| .birPattern _ => panic! "bir pattern in indexing" -- TODO
-
-def Access.interpFree : (a : Access) → LayoutMap a.freeDim
-| .simple s => simpleInterpFree s
-| .basic b => basicInterpFree b
-| .pattern p => patternInterpFree p
-| .birPattern _ => fun x => x -- TODO
-
-/-
-Execution of the compsed indexing
--/
-
-/-- Given an IndexSpan representing the parallel indicies of a composed query, construct an
-AccessBasic to extract those rows.
-
-TODO: Is s.extreme correct here? It's weird that we're forced to put in an (exclusive?) Nat bound
-in this representation, because it makes it impossible have a slice that decremenets to zero?
-
-The construction may need to be lifted to Err & exclude the "decrement down to 0" case.
--/
-def CompileIndex.par (t : TensorName) (s : IndexSpan) : AccessBasic where
-    tensor := t
-    indexes :=
-      let parIndex := .slice ⟨s.start, s.extreme, s.step, s.step_nz⟩
-      let freeIndices := t.shape.freeDims.map (.slice ∘ Slice.full)
-      parIndex :: freeIndices
-    lenWF := by simp
-
-/-- After applying all of your FreeSpans to a Layout you end up with another layout.
-Construct an AccessPattern that will extract these values from each row. -/
-def CompileIndex.freePairs (t : TensorName) (parNum : Nat) (l : Layout d) : AccessPattern where
-  tensor := t
-  parNum := parNum
-  freePattern := List.zipWith APPair.mk l.steps l.nums
-  freeOffset := l.offset
-
-def Layout.rowMajorForm (s : Shape) : Layout s.freeDim where
-  offset := 0
-  steps := s.freeDims.tails'.map <| Int.ofNat ∘ natListProd
-  nums := s.freeDims
-  steps_dim := by simp
-  nums_dim := by simp
+-- abbrev LayoutMap d := Layout d → Layout d
+--
+-- def coordToIndexSpan (x : Nat) : IndexSpan where
+--   start := x
+--   step := 1
+--   num := 1
+--   step_nz := Int.zero_ne_one.symm
+--   get_nonneg := by simp; omega
+--
+-- def Slice.toIndexSpan (s : Slice) (size : Nat) : IndexSpan where
+--   start := s.l
+--   step := s.step
+--   num := min size s.size
+--   step_nz := s.wf
+--   get_nonneg i := by
+--     suffices 0 ≤ i → i < ↑s.size → 0 ≤ ↑s.l + s.step * i by
+--       intro H1 H2; apply this H1
+--       apply Int.lt_of_lt_of_le H2
+--       apply Int.ofNat_le.mpr
+--       exact Nat.min_le_right size s.size
+--     simp [Slice.size]
+--     split <;> intros Hlb Hub
+--     · apply Int.le_add_of_neg_add_le_right
+--       rw [Int.neg_mul_eq_neg_mul, Int.add_zero]
+--       rw [← Int.toNat_of_nonneg Hlb] at Hub
+--       rw [Int.mul_comm]
+--       apply Int.mul_le_of_le_ediv; omega
+--       rw [← Int.max_eq_left Hlb, ← Int.ofNat_toNat]
+--       apply Int.le_trans (Int.le_of_lt Hub)
+--       rw [Int.natCast_ediv]
+--       apply Int.le_ediv_of_mul_le; omega
+--       have R1 : ↑s.step.natAbs = -s.step := by
+--         apply Int.ofNat_natAbs_of_nonpos; omega
+--       rw [R1]; clear R1
+--       apply Int.le_trans
+--       · apply Int.mul_le_mul_of_nonneg_right
+--         · apply Int.ediv_le_ediv
+--           · omega
+--           · apply Int.ofNat_le.mpr
+--             exact Nat.sub_le s.l s.u
+--         · omega
+--       apply Int.mul_le_of_le_ediv; omega
+--       apply Int.le_refl
+--     · rename_i h
+--       apply Int.add_nonneg (Int.ofNat_zero_le s.l)
+--       apply Int.mul_nonneg (Int.not_lt.mp h) Hlb
+--
+-- def Index.toIndexSpan (i : Index) (size : Nat) : IndexSpan :=
+--   match i with
+--   | .coord x => coordToIndexSpan x
+--   | .slice s => s.toIndexSpan size
+--
+-- def simpleInterpPar (t : TensorName) : IndexSpan :=
+--   .full t.shape.parDim
+--
+-- def simpleInterpFree (t : TensorName) : LayoutMap t.freeDim :=
+--   let F : FreeSpans t.freeDim := ⟨t.shape.freeDims.map .full, by simp⟩
+--   lcomp.comp F
+--
+-- def basicInterpPar (b : AccessBasic) : IndexSpan :=
+--   b.parIndex.toIndexSpan b.getShape.parDim
+--
+-- def basicInterpFree (b : AccessBasic) : LayoutMap b.freeDim :=
+--   let F : FreeSpans b.freeDim := FreeSpans.mk
+--     (List.zipWith (·.toIndexSpan ·) b.freeIndices b.getShape.freeDims)
+--     (by
+--       rcases b with ⟨_, L, Hwf⟩
+--       simp [AccessBasic.getShape, AccessBasic.shape]
+--       apply Nat.min_eq_right
+--       cases L
+--       · simp at Hwf
+--       · simp)
+--   lcomp.comp F
+--
+-- def patternInterpPar (p : AccessPattern) : IndexSpan :=
+--   .full p.parNum
+--
+-- def patternInterpFree (p : AccessPattern) : LayoutMap p.freeDim := fun l =>
+--   let coeff_sum : Int := (p.pattern.map APPair.step).sum
+--   Layout.mk
+--     (p.freeOffset + coeff_sum * l.offset).toNat
+--     (l.steps.map (coeff_sum * ·))
+--     (p.pattern.map APPair.num)
+--     l.offsets
+--     (by rw [List.length_map]; exact l.steps_dim)
+--     (by simp [List.length_map, AccessPattern.freeDim, AccessPattern.shape])
+--
+-- def Access.interpPar : Access → IndexSpan
+-- | .simple s => simpleInterpPar s
+-- | .basic b => basicInterpPar b
+-- | .pattern p => patternInterpPar p
+-- | .birPattern _ => panic! "bir pattern in indexing" -- TODO
+--
+-- def Access.interpFree : (a : Access) → LayoutMap a.freeDim
+-- | .simple s => simpleInterpFree s
+-- | .basic b => basicInterpFree b
+-- | .pattern p => patternInterpFree p
+-- | .birPattern _ => fun x => x -- TODO
+--
+-- /-
+-- Execution of the compsed indexing
+-- -/
+--
+-- /-- Given an IndexSpan representing the parallel indicies of a composed query, construct an
+-- AccessBasic to extract those rows.
+--
+-- TODO: Is s.extreme correct here? It's weird that we're forced to put in an (exclusive?) Nat bound
+-- in this representation, because it makes it impossible have a slice that decremenets to zero?
+--
+-- The construction may need to be lifted to Err & exclude the "decrement down to 0" case.
+-- -/
+-- def CompileIndex.par (t : TensorName) (s : IndexSpan) : AccessBasic where
+--     tensor := t
+--     indexes :=
+--       let parIndex := .slice ⟨s.start, s.extreme, s.step, s.step_nz⟩
+--       let freeIndices := t.shape.freeDims.map (.slice ∘ Slice.full)
+--       parIndex :: freeIndices
+--     lenWF := by simp
+--
+-- /-- After applying all of your FreeSpans to a Layout you end up with another layout.
+-- Construct an AccessPattern that will extract these values from each row. -/
+-- def CompileIndex.freePairs (t : TensorName) (parNum : Nat) (l : Layout d) : AccessPattern where
+--   tensor := t
+--   parNum := parNum
+--   pattern := (List.zip (List.zip l.steps l.nums) l.offsets).map (fun ((step, num), offset) => ⟨step, num, offset⟩)
+--   freeOffset := l.offset
+--
+-- def Layout.rowMajorForm (s : Shape) : Layout s.freeDim where
+--   offset := 0
+--   offsets := List.replicate s.freeDim 0
+--   steps := s.freeDims.tails'.map <| Int.ofNat ∘ natListProd
+--   nums := s.freeDims
+--   steps_dim := by simp
+--   nums_dim := by simp
 
 
 def TensorName.toAP (a : TensorName) : KLR.Err AccessPattern := do
@@ -666,7 +671,7 @@ def TensorName.toAP (a : TensorName) : KLR.Err AccessPattern := do
   return {
     tensor := a
     parNum := layout[0]!
-    freePattern := (List.zip steps layout).tail.map (fun (step, size) => ⟨step, size⟩)
+    pattern := (List.zip steps layout).map (fun (step, size) => ⟨step, size, 0⟩)
     freeOffset := 0
   }
 
@@ -685,13 +690,13 @@ private def getTensorName (shape : List Nat) : Err TensorName :=
   let t <- getTensorName [4,3,2]
   let ac <- TensorName.toAP t
   let bir := BirAccessPattern.fromAccessPattern ac
-  .ok (bir.pattern, bir.offset)) == .ok ([⟨6,4⟩, ⟨2,3⟩, ⟨1,2⟩], 0)
+  .ok (bir.pattern, bir.offset)) == .ok ([⟨6,4,0⟩, ⟨2,3,0⟩, ⟨1,2,0⟩], 0)
 
 #guard (do
   let t <- getTensorName [4,3]
   let ac <- TensorName.toAP t
   let bir := BirAccessPattern.fromAccessPattern ac
-  .ok (bir.pattern, bir.offset)) == .ok ([⟨3,4⟩, ⟨1,3⟩], 0)
+  .ok (bir.pattern, bir.offset)) == .ok ([⟨3,4,0⟩, ⟨1,3,0⟩], 0)
 
 
 def AccessBasic.idx_sz_and_offset (idxs : List Index) : List (Int × Int) :=
@@ -700,24 +705,21 @@ def AccessBasic.idx_sz_and_offset (idxs : List Index) : List (Int × Int) :=
       | .coord c => (1, c)
       | .slice s => (((s.u - s.l) / s.step), min s.l s.u))
 
-def idxToAp (layout : List Nat) (idxs : List Index) : (List APPair ×  Nat) :=
+def idxToAp (layout : List Nat) (idxs : List Index) : List APPair :=
   let steps := layout.tail ++ [1] -- step for dim 0 is 1 and the rest is prev dim
   let steps := steps.scanr (· * ·) 1 |>.dropLast -- actual step is accum of all prev step sizes
   let sz_off := AccessBasic.idx_sz_and_offset idxs -- get all index size and offset
-  let sz := sz_off.map (·.1.toNat)
-  let off := sz_off.map (·.2)
-  let totalOff := List.sum (List.zip off steps |>.map (fun (o, s) => o.toNat * s))
-  let pairs : List APPair :=  (List.zip steps sz).map (fun (st, sz) => ⟨ st, sz ⟩)
-  (pairs, totalOff)
+  let pairs : List APPair := List.zipWith (fun s (cnt, off) => ⟨s, cnt.toNat, off.toNat⟩) steps sz_off
+  pairs
 
 def AccessBasic.toAP (a : AccessBasic) : KLR.Err AccessPattern := do
   let layout := a.tensor.shape.toList
-  let (pairs, offset) := idxToAp layout a.indexes
+  let pairs := idxToAp layout a.indexes
   return {
     tensor := a.tensor
     parNum := pairs[0]!.num
-    freePattern := pairs.tail
-    freeOffset := offset
+    pattern := pairs
+    freeOffset := (pairs.map (fun x => x.offset)).sum
   }
 
 private def testAccess (idxs : List Index) : KLR.Err (List APPair × Nat) := do
@@ -736,31 +738,31 @@ private def testAccess (idxs : List Index) : KLR.Err (List APPair × Nat) := do
 
 #guard testAccess
  [.coord 0, .coord 0, .coord 0] ==
-  .ok ([⟨6,1⟩, ⟨2,1⟩, ⟨1,1⟩], 0)
+  .ok ([⟨6,1,0⟩, ⟨2,1,0⟩, ⟨1,1,0⟩], 0)
 #guard testAccess
  [.coord 0, .slice (Slice.make! 0 3 1), .slice (Slice.make! 0 2 1)] ==
-  .ok ([⟨6,1⟩, ⟨2,3⟩, ⟨1,2⟩], 0)
+  .ok ([⟨6,1,0⟩, ⟨2,3,0⟩, ⟨1,2,0⟩], 0)
 #guard testAccess
  [.coord 1, .slice (Slice.make! 0 3 1), .slice (Slice.make! 0 2 1)] ==
-  .ok ([⟨6,1⟩, ⟨2,3⟩, ⟨1,2⟩], 6)
+  .ok ([⟨6,1,1⟩, ⟨2,3,0⟩, ⟨1,2,0⟩], 6)
 #guard testAccess
  [.slice (Slice.make! 1 3 1), .slice (Slice.make! 0 3 1), .slice (Slice.make! 0 2 1)] ==
- .ok ([⟨6,2⟩, ⟨2,3⟩, ⟨1,2⟩], 6)
+ .ok ([⟨6,2,1⟩, ⟨2,3,0⟩, ⟨1,2,0⟩], 6)
 #guard testAccess
  [.slice (Slice.make! 0 4 1), .coord 0, .slice (Slice.make! 0 2 1)] ==
- .ok ([⟨6,4⟩, ⟨2,1⟩, ⟨1,2⟩], 0)
+ .ok ([⟨6,4,0⟩, ⟨2,1,0⟩, ⟨1,2,0⟩], 0)
 #guard testAccess
  [.slice (Slice.make! 0 4 1), .coord 1, .slice (Slice.make! 0 2 1)] ==
- .ok ([⟨6,4⟩, ⟨2,1⟩, ⟨1,2⟩], 2)
+ .ok ([⟨6,4,0⟩, ⟨2,1,1⟩, ⟨1,2,0⟩], 2)
 #guard testAccess
  [.slice (Slice.make! 0 4 1), .slice (Slice.make! 1 3 1), .slice (Slice.make! 0 2 1)] ==
- .ok ([⟨6,4⟩, ⟨2,2⟩, ⟨1,2⟩], 2)
+ .ok ([⟨6,4,0⟩, ⟨2,2,1⟩, ⟨1,2,0⟩], 2)
 #guard testAccess
  [.slice (Slice.make! 0 4 1), .slice (Slice.make! 0 3 1), .coord 0] ==
- .ok ([⟨6,4⟩, ⟨2,3⟩, ⟨1,1⟩], 0)
+ .ok ([⟨6,4,0⟩, ⟨2,3,0⟩, ⟨1,1,0⟩], 0)
 #guard testAccess
  [.slice (Slice.make! 0 4 1), .slice (Slice.make! 0 3 1), .coord 1] ==
- .ok ([⟨6,4⟩, ⟨2,3⟩, ⟨1,1⟩], 1)
+ .ok ([⟨6,4,0⟩, ⟨2,3,0⟩, ⟨1,1,1⟩], 1)
 
 def AccessPattern.toAP (a : AccessPattern) : KLR.Err AccessPattern :=
   .ok a
@@ -772,18 +774,31 @@ def Access.toAP (a : Access) : KLR.Err AccessPattern :=
   | .pattern p => .ok p
   | .birPattern _ => throw "Converting birAP to AP is lossy"
 
-def Access.combineAP (a : Access) (pat: List APPair) (offset : Nat) : KLR.Err AccessPattern := do
+def Access.combineAP (a : Access) (pat: List APPair) : KLR.Err AccessPattern := do
   let ap <- Access.toAP a
-  let pat1 := ⟨ap.freeDim, ap.parNum⟩ :: ap.freePattern
-  let off1 := ap.freeOffset
-  let pairs := List.zipWith (fun p1 p2 => ⟨max p1.step p2.step, min p1.num p2.num⟩) pat1 pat
-  let offset := off1 + offset
+  let pat1 := ap.pattern
+  let pairs := List.zipWith (fun p1 p2 => APPair.combine p1 p2) pat1 pat
   return {
     tensor := ap.tensor
     parNum := pairs[0]!.num
-    freePattern := pairs.tail
-    freeOffset := offset
+    pattern := pairs
+    freeOffset := pairs.foldl (fun acc p => acc + p.offset) 0
   }
+
+-- Normalize one AP in terms of the other. This is needed to resolve the fixed axis of one AP
+-- in terms of it's right axeses.
+--  E.g: in pattern `[1:3, 0, 1:3][1:2, 1:2]` the dimmension 1 is fixed and we will need to insert
+-- additional dimension when normalizing second access to align on dimmensions
+-- so second access `[(3,2), (1,2)]` becomes `[(3,2),(N, 1),(1,2)]` where N is the size of fixed
+-- dimmension from parent AP. We don't have to use N. But that would require special casing the
+-- combine operator for that stub value
+def Access.normWithAP (fixedAxis: List Nat) (this : List APPair) (pairs : List APPair) : List APPair :=
+  let rvPairs := pairs.mapIdx fun i pair =>
+    if fixedAxis.contains i then
+      { step := pair.step, num := 1, offset := 0 }
+    else
+      this[i - (fixedAxis.filter (· < i)).length]!
+  rvPairs
 
 def Access.combine (a : Access) (idx : List Index) : KLR.Err AccessPattern := do
   for i in idx do
@@ -794,9 +809,14 @@ def Access.combine (a : Access) (idx : List Index) : KLR.Err AccessPattern := do
       if s.step != 1 then
         throw "can't combine indecies with stride != 1"
     | _ => pure ()
+  let ap <- Access.toAP a
   let shape := <- a.shape
-  let (pat2, off2) := idxToAp shape.toList idx
-  Access.combineAP a pat2 off2
+  dbg_trace s!"{repr shape}"
+  let pat2 := idxToAp shape.toList idx
+  dbg_trace s!"idx {repr idx} to pairs {repr pat2}"
+  let pat2 := Access.normWithAP ap.fixedAxis pat2 ap.pattern
+  dbg_trace s!"pairs after norm {repr pat2}"
+  Access.combineAP a pat2
 
 private def testAccess2 (idxs1 : List Index) (idxs2 : List Index) : KLR.Err (List APPair × Nat) := do
   let addr : Address := {
@@ -811,17 +831,34 @@ private def testAccess2 (idxs1 : List Index) (idxs2 : List Index) : KLR.Err (Lis
   let bir := BirAccessPattern.fromAccessPattern ac2
   .ok (bir.pattern, bir.offset)
 
+#eval testAccess2
+    [.slice (Slice.make! 1 2 1), .slice (Slice.make! 0 3 1), .slice (Slice.make! 0 2 1)]
+    [.coord 0, .slice (Slice.make! 0 3 1), .coord 0]
+#eval testAccess2
+    [.slice (Slice.make! 1 2 1), .slice (Slice.make! 0 3 1), .slice (Slice.make! 0 2 1)]
+    [.coord 0, .slice (Slice.make! 1 2 1), .slice (Slice.make! 0 2 1)]
+#eval testAccess2
+    [.slice (Slice.make! 1 3 1), .slice (Slice.make! 1 3 1), .slice (Slice.make! 0 2 1)]
+    [.slice (Slice.make! 0 2 1), .slice (Slice.make! 1 2 1), .coord 1]
+#eval testAccess2
+    [.slice (Slice.make! 1 3 1), .slice (Slice.make! 1 3 1), .coord 1]
+    [.slice (Slice.make! 0 2 1), .slice (Slice.make! 0 2 1)]
+
 #guard testAccess2
     [.slice (Slice.make! 1 2 1), .slice (Slice.make! 0 3 1), .slice (Slice.make! 0 2 1)]
     [.coord 0, .slice (Slice.make! 0 3 1), .coord 0] ==
-    .ok ([⟨6,1⟩, ⟨2,3⟩, ⟨1,1⟩], 6)
+    .ok ([⟨6,1,1⟩, ⟨2,3,0⟩, ⟨1,1,0⟩], 6)
 #guard testAccess2
     [.slice (Slice.make! 1 2 1), .slice (Slice.make! 0 3 1), .slice (Slice.make! 0 2 1)]
     [.coord 0, .slice (Slice.make! 1 2 1), .slice (Slice.make! 0 2 1)] ==
-    .ok ([⟨6,1⟩, ⟨2,1⟩, ⟨1,2⟩], 8)
+    .ok ([⟨6,1,1⟩, ⟨2,1,0⟩, ⟨1,2,0⟩], 8)
 #guard testAccess2
     [.slice (Slice.make! 1 3 1), .slice (Slice.make! 1 3 1), .slice (Slice.make! 0 2 1)]
-    [.slice (Slice.make! 0 2 1), .slice (Slice.make! 0 2 1), .coord 1] ==
-     .ok ([⟨6,2⟩, ⟨2,2⟩, ⟨1,1⟩], 9)
+    [.slice (Slice.make! 0 2 1), .slice (Slice.make! 1 2 1), .coord 1] ==
+     .ok ([⟨6,2,1⟩, ⟨2,2,1⟩, ⟨1,1,1⟩], 11)
+#guard testAccess2
+    [.slice (Slice.make! 1 3 1), .slice (Slice.make! 1 3 1), .coord 1]
+    [.slice (Slice.make! 0 2 1), .slice (Slice.make! 0 2 1)] ==
+     .ok ([⟨6,2,1⟩, ⟨2,2,1⟩, ⟨1,1,1⟩], 11)
 
 end KLR.Core
